working/composition/event_based_refinement/load_balancer/compositional/abstract_composition/ComposedRefinementObligation.t.dfy
@@ -3,8 +3,6 @@ include "ComposedDistributedSystem.t.dfy"
 
 // analogous to module: RefinementTheorem
 abstract module ComposedRefinementTheorem refines ComposedDistributedSystem {
-    //import opened Types
-    //import opened DistributedSystem: ComposedDistributedSystem
 
     ghost function ConstantsAbstraction(c: Constants) : Spec.Constants
         requires c.WF()
@@ -22,20 +20,33 @@ abstract module ComposedRefinementTheorem refines ComposedDistributedSystem {
             Spec.DSB.VariablesAbstraction(c.dsB, v.dsB))
     }
 
+    ghost predicate InvMessages(c: Constants, v: Variables)
+    {
+        && (forall msg :: msg in v.network.sentMsgs && msg.MessageA? <==> msg.MessageA? && msg.msgA in v.dsA.network.sentMsgs)
+        && (forall msg :: msg in v.network.sentMsgs && msg.MessageB? <==> msg.MessageB? && msg.msgB in v.dsB.network.sentMsgs)
+    }
+
     ghost predicate Inv(c: Constants, v: Variables)
     {
         && Spec.DSA.Inv(c.dsA, v.dsA)
         && Spec.DSB.Inv(c.dsB, v.dsB)
+        && InvMessages(c, v)
     }
+
+    ghost predicate LiftedInv(c: Constants, v: Variables)
+
+    lemma LiftedInvLemma(c: Constants, v: Variables)
+        requires LiftedInv(c, v)
+        ensures Inv(c, v)
 
     lemma RefinementInit(c: Constants, v: Variables)
         requires Init(c, v)
-        ensures Inv(c, v)
+        ensures LiftedInv(c, v)
         ensures Spec.Init(ConstantsAbstraction(c), VariablesAbstraction(c, v))
     
-    lemma RefinementNext(c: Constants, v: Variables, v': Variables, evt: Option<Spec.Event>, step: Step)
-        requires NextStep(c, v, v', evt, step)
-        requires Inv(c, v)
-        ensures Inv(c, v') 
+    lemma RefinementNext(c: Constants, v: Variables, v': Variables, evt: Option<Spec.Event>)
+        requires Next(c, v, v', evt)
+        requires LiftedInv(c, v)
+        ensures LiftedInv(c, v') 
         ensures (evt.Some? && Spec.Next(ConstantsAbstraction(c), VariablesAbstraction(c, v), VariablesAbstraction(c, v'), evt.value)) || (evt.None? && VariablesAbstraction(c, v) == VariablesAbstraction(c, v'))
 }
