working/composition/event_based_refinement/load_balancer/compositional/client/DistributedSystem.v.dfy
@@ -4,14 +4,9 @@ include "Network.v.dfy"
 module ClientDistributedSystem refines RefinementTheorem {
     import opened Network = ClientNetwork
 
-    ghost predicate ValidStep(c: Constants, v: Variables, v': Variables, evt: Option<Host.Spec.Event>)
+    ghost predicate ValidNext(c: Constants, v: Variables, v': Variables)
     {
-        exists msgOps :: NextStep(c, v, v', evt, HostActionStep(0, msgOps))
-    }
-
-    ghost predicate NoOp(c: Constants, v: Variables, v': Variables)
-    {
-        exists msgOps :: NextStep(c, v, v', None, HostActionStep(0, msgOps))
+        exists evt :: Next(c, v, v', evt)
     }
 
     ghost predicate NonTriviality_Part1Spec(c: Constants, behavior: seq<Variables>)
@@ -19,12 +14,10 @@ module ClientDistributedSystem refines RefinementTheorem {
         && c.WF()
         && 0 < |behavior|
         && Init(c, behavior[0])
-        && (forall i:nat | i < |behavior|-1 :: 
-            (|| ValidStep(c, behavior[i], behavior[i+1], None) 
-            || ValidStep(c, behavior[i], behavior[i+1], Some(Network.Host.Spec.SendRequest)) 
-            || ValidStep(c, behavior[i], behavior[i+1], Some(Network.Host.Spec.ReceiveResponse))))
+        && (forall i:nat | 0 <= i < |behavior|-1 :: ValidNext(c, behavior[i], behavior[i+1]))
         && behavior[|behavior|-1].WF(c) 
         && |behavior[|behavior|-1].hosts[0].requests| == 1
+        && |behavior[|behavior|-1].hosts[0].responses| == 0
     }
 
     lemma NonTriviality_Part1(c: Constants) returns (behavior: seq<Variables>)
@@ -49,6 +42,7 @@ module ClientDistributedSystem refines RefinementTheorem {
         )];
         assert Host.SendRequest(c.hosts[0], behavior[0].hosts[0], behavior[1].hosts[0], Some(Host.Spec.SendRequest), msgOps);
         assert NextStep(c, behavior[0], behavior[1], Some(Host.Spec.SendRequest), HostActionStep(0, msgOps));
+        assert Next(c, behavior[0], behavior[1], Some(Host.Spec.SendRequest));
     }
 
     ghost predicate ExistsCorrectClientResponse(c: Constants, part2: seq<Variables>, i: nat, request: ServiceRequest<(int, int)>)
@@ -73,7 +67,7 @@ module ClientDistributedSystem refines RefinementTheorem {
         && |part1| < |part2|
         && part2[0..|part1|] == part1
         && 0 < |part2[|part1|..]|
-        && (forall i:nat | |part1| <= i < |part2| - 1 :: NoOp(c, part2[i], part2[i+1]))
+        && (forall i:nat | |part1| <= i < |part2| - 1 :: Next(c, part2[i], part2[i+1], None))
         && (forall i:nat | |part1| <= i < |part2| - 1 :: part2[i].hosts == part1[|part1|-1].hosts)
         && (ExistsCorrectClientResponse(c, part2, |part2| - 2, part1[|part1|-1].hosts[0].requests[0]))
     }
@@ -84,14 +78,12 @@ module ClientDistributedSystem refines RefinementTheorem {
         && |part2| < |part3|
         && part3[0..|part2|] == part2
         && 0 < |part3[|part2|..]|
-        && (forall i:nat | |part2| <= i < |part3|-1 :: 
-            (|| ValidStep(c, part3[i], part3[i+1], None) 
-            || ValidStep(c, part3[i], part3[i+1], Some(Network.Host.Spec.SendRequest)) 
-            || ValidStep(c, part3[i], part3[i+1], Some(Network.Host.Spec.ReceiveResponse))))
+        && (forall i:nat | |part2| <= i < |part3|-1 :: ValidNext(c, part3[i], part3[i+1]))
         && part3[|part3|-1].WF(c)
+        && |part3[|part3|-1].hosts[0].requests| == 1
         && |part3[|part3|-1].hosts[0].responses| == 1
-        && part3[|[part3]|-1].hosts[0].responses[0].seqNo == part3[|part3|-1].hosts[0].requests[0].seqNo
-        && part3[|[part3]|-1].hosts[0].responses[0].val == part3[|part3|-1].hosts[0].requests[0].val.0 + part3[|part3|-1].hosts[0].requests[0].val.1
+        //&& part3[|[part3]|-1].hosts[0].responses[0].seqNo == part3[|part3|-1].hosts[0].requests[0].seqNo
+        //&& part3[|[part3]|-1].hosts[0].responses[0].val == part3[|part3|-1].hosts[0].requests[0].val.0 + part3[|part3|-1].hosts[0].requests[0].val.1
     }
 
     lemma NonTriviality_Part3(c: Constants, part1: seq<Variables>, part2: seq<Variables>) returns (behavior: seq<Variables>)
@@ -102,7 +94,6 @@ module ClientDistributedSystem refines RefinementTheorem {
         behavior := part2;
 
         var msgOps :| CorrectClientResponse(c, part2, |part2| - 2, part2[|part2|-1].hosts[0].requests[0], msgOps);
-        assert msgOps.send.Some?;
         var recv := msgOps.send.value;
         msgOps := Host.MessageOps(Some(recv), None);
         var clientResp := recv.response;
@@ -112,7 +103,8 @@ module ClientDistributedSystem refines RefinementTheorem {
             ],
             part2[|part2|-1].network
         )];
-        assert Host.ReceiveResponse(c.hosts[0], behavior[4].hosts[0], behavior[5].hosts[0], Some(Host.Spec.ReceiveResponse), msgOps);
-        assert NextStep(c, behavior[4], behavior[5], Some(Host.Spec.ReceiveResponse), HostActionStep(0, msgOps));
+        var i := |behavior| - 2;
+        assert Host.ReceiveResponse(c.hosts[0], behavior[i].hosts[0], behavior[i+1].hosts[0], Some(Host.Spec.ReceiveResponse), msgOps);
+        assert NextStep(c, behavior[i], behavior[i+1], Some(Host.Spec.ReceiveResponse), HostActionStep(0, msgOps));
     }
 }
