working/composition/event_based_refinement/load_balancer/compositional/client_server/ClientServerDistributedSystem.v.dfy
@@ -3,4 +3,98 @@ include "ClientServerNetwork.v.dfy"
 
 module ClientServerDistributedSystem refines ComposedRefinementTheorem {
     import opened Network = ClientServerNetwork
+
+    ghost predicate ValidNext(c: Constants, v: Variables, v': Variables)
+    {
+        exists evt :: Next(c, v, v', evt)
+    }
+
+    lemma NonTriviality(c: Constants) returns (behavior: seq<Variables>)
+        requires c.WF()
+        ensures 0 < |behavior|
+        ensures Init(c, behavior[0])
+        ensures forall i:nat | i < |behavior|-1 :: ValidNext(c, behavior[i], behavior[i+1])
+        ensures behavior[|behavior|-1].WF(c)
+        ensures |behavior[|behavior|-1].dsA.hosts[0].requests| == |behavior[|behavior|-1].dsA.hosts[0].responses| == 1
+        ensures behavior[|behavior|-1].dsA.hosts[0].responses[0].val == behavior[|behavior|-1].dsA.hosts[0].requests[0].val.0 + behavior[|behavior|-1].dsA.hosts[0].requests[0].val.1
+        {
+            // Init
+            behavior := [Variables.Variables(
+                Spec.DSA.Variables([Spec.DSA.Network.Host.Variables([], [])], Spec.DSA.Network.Variables({})),
+                Spec.DSB.Variables([Spec.DSB.Network.Host.Variables([], [])], Spec.DSB.Network.Variables({})),
+                Network.Variables({})
+            )];
+
+            // SendRequest (client)
+            var req := ServiceRequest(0, (4, 5));
+            var sentA := Spec.DSA.Network.Host.ClientRequest(req);
+            var sentB := Spec.DSB.Network.Host.ServerRequest(req);
+            var sent := MessageA(sentA);
+            var sentTrans := MessageB(sentB);
+            var msgOps := Network.MessageOps(None, Some(sent), Some(sentTrans));
+            var msgOpsA := Spec.DSA.Network.Host.MessageOps(None, Some(sentA));
+            var event := Some(Spec.EventA(Spec.DSA.Network.Host.Spec.SendRequest));
+            var eventA := Some(Spec.DSA.Network.Host.Spec.SendRequest);
+            behavior := behavior + [Variables.Variables(
+                Spec.DSA.Variables([Spec.DSA.Network.Host.Variables([req], [])], Spec.DSA.Network.Variables({ sentA })),
+                Spec.DSB.Variables([Spec.DSB.Network.Host.Variables([], [])], Spec.DSB.Network.Variables({ sentB })),
+                Network.Variables({ sent, sentTrans })
+            )];
+            assert Spec.DSA.Network.Host.SendRequest(c.dsA.hosts[0], behavior[0].dsA.hosts[0], behavior[1].dsA.hosts[0], eventA, msgOpsA);
+            assert Spec.DSA.NextStep(c.dsA, behavior[0].dsA, behavior[1].dsA, eventA, Spec.DSA.HostActionStep(0, msgOpsA));
+            assert UnwrapEventA(event) == eventA;
+            assert UnwrapMessageOpsA(msgOps) == msgOpsA;
+            assert DSAAction(c, behavior[0], behavior[1], event, msgOps);
+            assert DSAction(c, behavior[0], behavior[1], event, msgOps);
+            assert NextStep(c, behavior[0], behavior[1], event, DSActionStep(msgOps));
+            assert Next(c, behavior[0], behavior[1], event);
+
+            // Compute (server)
+            var recv := msgOps.send_trans.value;
+            var recvB := recv.msgB;
+            var sum := recvB.request.val.0 + recvB.request.val.1;
+            var resp := ServiceResponse(recvB.request.seqNo, sum);
+            var sentB2 := Spec.DSB.Network.Host.ServerResponse(resp);
+            var sentA2 := Spec.DSA.Network.Host.ClientResponse(resp);
+            var sent2 := MessageB(sentB2);
+            var sentTrans2 := MessageA(sentA2);
+            var msgOpsB := Spec.DSB.Network.Host.MessageOps(Some(recvB), Some(sentB2));
+            msgOps := Network.MessageOps(Some(recv), Some(sent2), Some(sentTrans2));
+            event := Some(Spec.EventB(Spec.DSB.Network.Host.Spec.Compute));
+            var eventB := Some(Spec.DSB.Network.Host.Spec.Compute);
+            behavior := behavior + [Variables.Variables(
+                Spec.DSA.Variables([Spec.DSA.Network.Host.Variables([req], [])], Spec.DSA.Network.Variables({ sentA, sentA2 })),
+                Spec.DSB.Variables([Spec.DSB.Network.Host.Variables([req], [resp])], Spec.DSB.Network.Variables({ sentB, sentB2 })),
+                Network.Variables({ sent, sentTrans, sent2, sentTrans2 })
+            )];
+            assert Spec.DSB.Network.Host.Compute(c.dsB.hosts[0], behavior[1].dsB.hosts[0], behavior[2].dsB.hosts[0], eventB, msgOpsB);
+            assert Spec.DSB.NextStep(c.dsB, behavior[1].dsB, behavior[2].dsB, eventB, Spec.DSB.HostActionStep(0, msgOpsB));
+            assert UnwrapEventB(event) == eventB;
+            assert UnwrapMessageOpsB(msgOps) == msgOpsB;
+            assert DSBAction(c, behavior[1], behavior[2], event, msgOps);
+            assert DSAction(c, behavior[1], behavior[2], event, msgOps);
+            assert NextStep(c, behavior[1], behavior[2], event, DSActionStep(msgOps));
+            assert Next(c, behavior[1], behavior[2], event);
+
+            // ReceiveResponse (client)
+            recv := msgOps.send_trans.value;
+            var recvA := recv.msgA;
+            msgOpsA := Spec.DSA.Network.Host.MessageOps(Some(recvA), None);
+            msgOps := Network.MessageOps(Some(recv), None, None);
+            event := Some(Spec.EventA(Spec.DSA.Network.Host.Spec.ReceiveResponse));
+            eventA := Some(Spec.DSA.Network.Host.Spec.ReceiveResponse);
+            behavior := behavior + [Variables.Variables(
+                Spec.DSA.Variables([Spec.DSA.Network.Host.Variables([req], [resp])], Spec.DSA.Network.Variables({ sentA, sentA2 })),
+                Spec.DSB.Variables([Spec.DSB.Network.Host.Variables([req], [resp])], Spec.DSB.Network.Variables({ sentB, sentB2 })),
+                Network.Variables({ sent, sentTrans, sent2, sentTrans2 })
+            )];
+            assert Spec.DSA.Network.Host.ReceiveResponse(c.dsA.hosts[0], behavior[2].dsA.hosts[0], behavior[3].dsA.hosts[0], eventA, msgOpsA);
+            assert Spec.DSA.NextStep(c.dsA, behavior[2].dsA, behavior[3].dsA, eventA, Spec.DSA.HostActionStep(0, msgOpsA));
+            assert UnwrapEventA(event) == eventA;
+            assert UnwrapMessageOpsA(msgOps) == msgOpsA;
+            assert DSAAction(c, behavior[2], behavior[3], event, msgOps);
+            assert DSAction(c, behavior[2], behavior[3], event, msgOps);
+            assert NextStep(c, behavior[2], behavior[3], event, DSActionStep(msgOps));
+            assert Next(c, behavior[2], behavior[3], event);
+        }
 }
