working/composition/event_based_refinement/load_balancer/compositional/client_server/ClientServerRefinementProof.v.dfy
@@ -2,18 +2,50 @@ include "../abstract_composition/ComposedRefinementObligation.t.dfy"
 include "ClientServerDistributedSystem.v.dfy"
 
 module ClientServerRefinementProof refines ClientServerDistributedSystem {
+
+    ghost predicate Inv_ServerRequestClientRequest(c: Constants, v: Variables) 
+        requires v.WF(c)
+    {
+        forall msg :: 
+            && msg in v.network.sentMsgs 
+            && msg.MessageB?
+            && msg.msgB.ServerRequest? ==> 
+            MessageA(Spec.DSA.Network.Host.ClientRequest(msg.msgB.request)) in v.network.sentMsgs
+    }
+
+    ghost predicate Inv_ServerResponseClientResponse(c: Constants, v: Variables) 
+        requires v.WF(c)
+    {
+        forall msg :: 
+            && msg in v.network.sentMsgs 
+            && msg.MessageA?
+            && msg.msgA.ClientResponse? ==> 
+            MessageB(Spec.DSB.Network.Host.ServerResponse(msg.msgA.response)) in v.network.sentMsgs
+    }
+
+    ghost predicate LiftedInv(c: Constants, v: Variables)
+    {
+        && Inv(c, v)
+        && Inv_ServerRequestClientRequest(c, v)
+        && Inv_ServerResponseClientResponse(c, v)
+    }
+
+    lemma LiftedInvLemma(c: Constants, v: Variables)
+        // requires LiftedInv(c, v)
+        // ensures Inv(c, v)
+    {}
     
     lemma RefinementInit(c: Constants, v: Variables)
 //        requires DistributedSystem.Init(c, v)
-//        ensures Inv(c, v)
+//        ensures LiftedInv(c, v)
 //        ensures Spec.Init(ConstantsAbstraction(c), VariablesAbstraction(c, v))
     {
     }
 
-    lemma RefinementNext(c: Constants, v: Variables, v': Variables, evt: Option<Spec.Event>, step: Step)
-//        requires DistributedSystem.NextStep(c, v, v', evt, step)
-//        requires Inv(c, v)
-//        ensures Inv(c, v') 
+    lemma RefinementNext(c: Constants, v: Variables, v': Variables, evt: Option<Spec.Event>)
+//        requires DistributedSystem.Next(c, v, v', evt)
+//        requires LiftedInv(c, v)
+//        ensures LiftedInv(c, v') 
 //        ensures Spec.Next(ConstantsAbstraction(c), VariablesAbstraction(c, v), VariablesAbstraction(c, v'), evt) || (VariablesAbstraction(c, v) == VariablesAbstraction(c, v') && evt == NoOp)
     {
     }
