working/composition/event_based_refinement/load_balancer/compositional/server/DistributedSystem.v.dfy
@@ -4,4 +4,104 @@ include "Network.v.dfy"
 
 module ServerDistributedSystem refines RefinementTheorem {
     import opened Network = ServerNetwork
+
+    ghost predicate ValidNext(c: Constants, v: Variables, v': Variables)
+    {
+        exists evt, step: Step :: NextStep(c, v, v', evt, step)
+    }
+
+    ghost predicate NetworkStep(c: Constants, v: Variables, v': Variables, evt: Option<Host.Spec.Event>)
+    {
+        exists step: Step :: step.NetworkActionStep? && NetworkAction(c, v, v', evt, step.msgOps)
+    }
+
+    ghost predicate ExistsRequestMessage(c: Constants, prefix: seq<Variables>, i: nat)
+        requires |prefix| > i + 1
+    {
+        exists msgOps :: RequestMessage(c, prefix, i, msgOps)
+    }
+
+    ghost predicate RequestMessage(c: Constants, prefix: seq<Variables>, i: nat, msgOps: Host.MessageOps)
+        requires |prefix| > i + 1
+    {
+        && NetworkAction(c, prefix[i], prefix[i+1], None, msgOps) 
+        && msgOps.send.Some?
+        && msgOps.send.value.ServerRequest?
+        && msgOps.send.value.request.seqNo == 0
+    }
+
+    ghost predicate NonTriviality_PrefixSpec(c: Constants, prefix: seq<Variables>)
+    {
+        && c.WF()
+        && 1 < |prefix|
+        && Init(c, prefix[0])
+        && (forall i:nat | 0 <= i < |prefix| - 1 :: NetworkStep(c, prefix[i], prefix[i+1], None))
+        && ExistsRequestMessage(c, prefix, |prefix| - 2)
+    }
+
+    ghost predicate NonTriviality_Spec(c: Constants, prefix: seq<Variables>, behavior: seq<Variables>)
+    {
+        && NonTriviality_PrefixSpec(c, prefix)
+        && |prefix| < |behavior|
+        && behavior[0..|prefix|] == prefix
+        && (forall i:nat | 0 <= i < |behavior|-1 :: ValidNext(c, behavior[i], behavior[i+1]))
+        && behavior[|behavior|-1].WF(c) 
+        && |behavior[|behavior|-1].hosts[0].requests| == |behavior[|behavior|-1].hosts[0].responses| == 1
+    }
+
+    lemma NoOpsPreserveState(c: Constants, start: nat, behavior: seq<Variables>)
+        requires forall i:nat | start <= i < |behavior| - 1 :: NetworkStep(c, behavior[i], behavior[i+1], None)
+        requires |behavior| - start >= 2
+        decreases |behavior| - start
+        ensures forall i, j: nat | start <= i < j < |behavior| - 1 :: behavior[i].hosts ==  behavior[j].hosts
+    {
+        assert behavior[start].hosts == behavior[start+1].hosts;
+        if (|behavior| - start > 2)
+        {
+            NoOpsPreserveState(c, start + 1, behavior);
+        }
+    }
+
+    lemma NetworkStepsAreValidSteps(c: Constants, behavior: seq<Variables>)
+        requires forall i:nat | 0 <= i < |behavior| - 1 :: NetworkStep(c, behavior[i], behavior[i+1], None)
+        requires 1 < |behavior|
+        ensures forall i:nat | 0 <= i < |behavior| - 1 :: ValidNext(c, behavior[i], behavior[i+1])
+    {
+        assert NetworkStep(c, behavior[0], behavior[1], None);
+        var step: Step :| step.NetworkActionStep? && NetworkAction(c, behavior[0], behavior[1], None, step.msgOps);
+        assert NextStep(c, behavior[0], behavior[1], None, step);
+        if (|behavior| > 2) {
+            NetworkStepsAreValidSteps(c, behavior[1..]);
+        }
+    }
+
+    lemma NonTriviality(c: Constants, prefix: seq<Variables>) returns (behavior: seq<Variables>)
+        requires c.WF()
+        requires NonTriviality_PrefixSpec(c, prefix)
+        ensures NonTriviality_Spec(c, prefix, behavior)
+    {
+        behavior := prefix;
+        NetworkStepsAreValidSteps(c, behavior);
+        assert (forall i:nat | 0 <= i < |behavior| - 1 :: ValidNext(c, behavior[i], behavior[i+1]));
+
+        var msgOps :| RequestMessage(c, prefix, |prefix| - 2, msgOps);
+        var recv := msgOps.send.value;
+        var sum := recv.request.val.0 + recv.request.val.1;
+        var resp := ServiceResponse(recv.request.seqNo, sum);
+        var sent := Host.ServerResponse(resp);
+        msgOps := Host.MessageOps(Some(recv), Some(sent));
+        behavior := behavior + [Variables.Variables(
+            [
+                Host.Variables([recv.request], [resp])
+            ],
+            Network.Variables(prefix[|prefix|-1].network.sentMsgs + {sent})
+        )];
+        var i := |behavior| - 2;
+        NoOpsPreserveState(c, 0, prefix);
+        assert |prefix[i].hosts[0].requests| == |prefix[i].hosts[0].responses| == 0;
+        assert prefix[i] == behavior[i];
+        assert Host.Compute(c.hosts[0], behavior[i].hosts[0], behavior[i+1].hosts[0], Some(Host.Spec.Compute), msgOps);
+        assert NextStep(c, behavior[i], behavior[i+1], Some(Host.Spec.Compute), HostActionStep(0, msgOps));
+        assert Next(c, behavior[i], behavior[i+1], Some(Host.Spec.Compute));
+    }
 }
