working/composition/event_based_refinement/load_balancer/compositional/shared/RefinementObligation.t.dfy
@@ -2,8 +2,6 @@ include "Types.t.dfy"
 include "DistributedSystem.t.dfy"
 
 abstract module RefinementTheorem refines AbstractDistributedSystem {
-    //import opened Types
-    //import opened DistributedSystem: AbstractDistributedSystem
 
     ghost function ConstantsAbstraction(c: Constants) : Network.Host.Spec.Constants
         requires c.WF()
@@ -13,13 +11,22 @@ abstract module RefinementTheorem refines AbstractDistributedSystem {
 
     ghost predicate Inv(c: Constants, v: Variables)
 
+    lemma InvInductiveBase(c: Constants, v: Variables)
+        requires Init(c, v)
+        ensures Inv(c, v)
+
+    lemma InvInductiveNext(c: Constants, v: Variables, v': Variables, evt: Option<Network.Host.Spec.Event>)
+        requires Next(c, v, v', evt)
+        requires Inv(c, v)
+        ensures Inv(c, v')
+
     lemma RefinementInit(c: Constants, v: Variables)
         requires Init(c, v)
         ensures Inv(c, v)
         ensures Network.Host.Spec.Init(ConstantsAbstraction(c), VariablesAbstraction(c, v))
     
-    lemma RefinementNext(c: Constants, v: Variables, v': Variables, evt: Option<Network.Host.Spec.Event>, step: Step)
-        requires NextStep(c, v, v', evt, step)
+    lemma RefinementNext(c: Constants, v: Variables, v': Variables, evt: Option<Network.Host.Spec.Event>)
+        requires Next(c, v, v', evt)
         requires Inv(c, v)
         ensures Inv(c, v') 
         ensures (evt.Some? && Network.Host.Spec.Next(ConstantsAbstraction(c), VariablesAbstraction(c, v), VariablesAbstraction(c, v'), evt.value)) || (evt.None? && VariablesAbstraction(c, v) == VariablesAbstraction(c, v'))
